Matroid/Connectivity/Fan/Circuit.lean
@@ -788,7 +788,7 @@ lemma foo {M : Matroid α} {F : List α} (hF : M.IsFan F true false)
     (hT : M.IsTriad {F[F.length - 2], F[F.length - 1], F[0]})
     (hconn : (M ＼ {F[0]}).Connected) : M.IsTriangle {F[F.length - 1], F[0], F[1]} := by
   obtain ⟨n, hn⟩ : ∃ n, F.length = 2 * n + 4 := sorry
-
+  simp only [hn, Nat.reduceSubDiff, Nat.add_one_sub_one] at hT ⊢
   have hF4 : 4 ≤ F.length := sorry
 
   have hE : M.E = {e | e ∈ F} := by
@@ -801,14 +801,21 @@ lemma foo {M : Matroid α} {F : List α} (hF : M.IsFan F true false)
         rfl (by simp) hC.1 (by grind) h1C h1
       simp only [hC_eq, zero_add, altBetween, exists_and_left, Set.mem_insert_iff] at hxC
       grind
-    simp only [hn, Nat.reduceSubDiff, Nat.add_one_sub_one] at hT
     rw [hT.reverse.mem_iff_mem_of_isCocircuit (by simpa using hC.1) hC.2] at h1
     obtain ⟨j, _, _, _, rfl⟩ :=
       hF.exists_eq_interval_of_notMem_mem_add_one (i := 0) (t := 2 * n + 2) (C := C)
       (by lia) (by lia) rfl (by simp) hC.1 hC.2 h1C h1
     simp only [zero_add, altBetween, Bool.not_true, exists_and_left, Set.mem_insert_iff] at hxC
     grind
-  by_cases hpara : (M ／ {F[0]}).Paralle
+  have := hF.dual.joints_indep'' (by simp)
+  -- have hnp : ¬M.Parallel F[1] F[2 * n + 3] := by
+  --   intro hC
+  --   simpa [hF.nodup.getElem_inj_iff] using hT.isCocircuit.mem_iff_mem_of_parallel hC
+  -- rw [pair_comm, insert_comm, isTriangle_iff_parallel_contract hnp]
+  -- by_contra hcon
+  -- have := (hF.tail (by lia)).contract_disjoint (X := {F[0]})
+  -- by_cases hpara : (M ／ {F[0]}).Parallel F[2 * n + 3] F[1]
+  -- · rw [parallel_iff_isCircuit (by simp [hF.nodup.getElem_inj_iff])] at hpara
 
     -- rw [← hF.mem_iff_mem₁₂] at h1
     -- have := hF.exists_eq_interval_of_notMem_mem_add_one (i := 0) ()
